metatheory/metaTerminationScript.sml
@@ -1,0 +1,21 @@
+open preamble 
+open TypeSoundInvariantsTheory BigSmallInvariantsTheory;
+
+val _ = new_theory "metaTermination";
+
+fun register name def ind =
+  let val _ = save_thm (name ^ "_def", def);
+      val _ = save_thm (name ^ "_ind", ind);
+      val _ = computeLib.add_persistent_funs [name ^ "_def"];
+  in
+    ()
+  end
+
+val (consistent_mod_env_def, consistent_mod_env_ind) =
+  tprove_no_defn ((consistent_mod_env_def, consistent_mod_env_ind),
+  WF_REL_TAC `measure (λ(a,b,c,d). LENGTH c)` >>
+  rw []);
+val _ = register "consistent_mod_env" consistent_mod_env_def consistent_mod_env_ind;
+val _ = export_rewrites["consistent_mod_env_def"];
+
+val _ = export_theory ();
