semantics/terminationScript.sml
@@ -1,5 +1,5 @@
 open preamble intSimps;
-open LibTheory AstTheory SemanticPrimitivesTheory TypeSystemTheory;
+open LibTheory AstTheory SemanticPrimitivesTheory TypeSystemTheory AltBigStepTheory;
 
 val _ = new_theory "termination";
 
@@ -78,14 +78,12 @@ val (pmatch_def, pmatch_ind) =
                              | INR (s,a,ps,b,c) => pat1_size ps)`);
 val _ = register "pmatch" pmatch_def pmatch_ind;
 
-(*
 val (pmatch'_def, pmatch'_ind) =
   tprove_no_defn ((pmatch'_def, pmatch'_ind),
   wf_rel_tac
   `inv_image $< (λx. case x of INL (s,p,b,c) => pat_size p
                              | INR (s,ps,b,c) => pat1_size ps)`);
 val _ = register "pmatch'" pmatch'_def pmatch'_ind;
-*)
 
 val (contains_closure_def, contains_closure_ind) =
   tprove_no_defn ((contains_closure_def, contains_closure_ind),
